refactor(examples): use IMP2 notation

src/Examples/Interprocedural/Example_Inc_Proc.thy
@@ -22,15 +22,15 @@ definition inc_pi :: proc_table where
 
 lemma inc_program_parts:
   shows "prog_procs inc_program = [''p'']"
-    and "prog_table inc_program = (\<lambda>_. None)(''p'' := Some (proc_decl_of [] (Assign ''Gx'' (Plus (V ''Gx'') (N 1)))))"
-    and "prog_main inc_program = Call None ''p'' []"
+    and "prog_table inc_program = map_of [(''p'', proc_decl_of [] (imp \<lbrakk> Gx := Gx + 1 \<rbrakk>))]"
+    and "prog_main inc_program = imp \<lbrakk> p() \<rbrakk>"
   by (simp_all add: inc_program_def)
 
 definition inc_g :: cfg where
-  "inc_g = compile_prog (prog_table inc_program) (prog_procs inc_program) (prog_main inc_program)"
+  "inc_g = compile_prog (prog_table inc_program) (prog_procs inc_program) ''main'' (prog_main inc_program)"
 
 lemma inc_g_eq_compile:
-  "inc_g = compile_prog inc_pi [''p''] (Call None ''p'' [])"
+  "inc_g = compile_prog inc_pi [''p''] ''main'' (imp \<lbrakk> p() \<rbrakk>)"
   by (simp add: inc_g_def inc_pi_def inc_program_parts)
 
 lemma inc_g_full:
@@ -68,11 +68,11 @@ lemma combine_after_enter_global_assign:
 
 lemma pcompletes_inc_pcall:
   fixes s :: store
-  shows "pcompletes inc_pi (Call None ''p'' []) s (s(''Gx'' := s ''Gx'' + 1))"
+  shows "pcompletes inc_pi (imp \<lbrakk> p() \<rbrakk>) s (s(''Gx'' := s ''Gx'' + 1))"
 proof -
-  let ?body = "Assign ''Gx'' (Plus (V ''Gx'') (N 1))"
+  let ?body = "imp \<lbrakk> Gx := Gx + 1 \<rbrakk>"
   have g: "is_global ''Gx''" by (simp add: is_global_def)
-  have run: "pcompletes inc_pi (Call None ''p'' []) s
+  have run: "pcompletes inc_pi (imp \<lbrakk> p() \<rbrakk>) s
                 (<s | (enter_state s)(''Gx'' := s ''Gx'' + 1)>)"
   proof (rule pcompletes_Call_parameterless[where c = ?body])
     show "inc_pi ''p'' = Some (proc_decl_of [] ?body)"
