src/Examples/Interprocedural/Example_Mixed_Flow_Sign.thy
@@ -38,51 +38,51 @@ definition sign_init_s0 :: "sign abs_state" where
 corollary sign_mixed_flow_sound_and_optimal:
   fixes S :: "store set"
   assumes dom:
-    "side_cfg_solve_dom_eff (compile_prog inc_pi [''p''] (IMP2_Proc.Call None ''p'' []))
+    "side_cfg_solve_dom_eff (compile_prog inc_pi [''p''] (imp \<lbrakk> p() \<rbrakk>))
        sign_etf bot sign_init_s0 ()
-       (cfg_exit (compile_prog inc_pi [''p''] (IMP2_Proc.Call None ''p'' [])))"
+       (cfg_exit (compile_prog inc_pi [''p''] (imp \<lbrakk> p() \<rbrakk>)))"
   assumes S_sound: "S \<le> \<lbrakk>sign_init_s0\<rbrakk>"
   shows
-    "ltr_collect (compile_prog inc_pi [''p''] (IMP2_Proc.Call None ''p'' [])) S
-       (cfg_exit (compile_prog inc_pi [''p''] (IMP2_Proc.Call None ''p'' [])))
-     \<le> \<lbrakk>side_analyse_eff inc_pi [''p''] (IMP2_Proc.Call None ''p'' []) sign_etf
+    "ltr_collect (compile_prog inc_pi [''p''] (imp \<lbrakk> p() \<rbrakk>)) S
+       (cfg_exit (compile_prog inc_pi [''p''] (imp \<lbrakk> p() \<rbrakk>)))
+     \<le> \<lbrakk>side_analyse_eff inc_pi [''p''] (imp \<lbrakk> p() \<rbrakk>) sign_etf
           bot sign_init_s0 ()
-          (cfg_exit (compile_prog inc_pi [''p''] (IMP2_Proc.Call None ''p'' [])))\<rbrakk>"
+          (cfg_exit (compile_prog inc_pi [''p''] (imp \<lbrakk> p() \<rbrakk>)))\<rbrakk>"
     and
     "least_part_post_solution
-       (side_cfg_T_eff (compile_prog inc_pi [''p''] (IMP2_Proc.Call None ''p'' []))
+       (side_cfg_T_eff (compile_prog inc_pi [''p''] (imp \<lbrakk> p() \<rbrakk>))
           sign_etf bot sign_init_s0 ())
-       (cfg_exit (compile_prog inc_pi [''p''] (IMP2_Proc.Call None ''p'' [])))
+       (cfg_exit (compile_prog inc_pi [''p''] (imp \<lbrakk> p() \<rbrakk>)))
        (td_cfg_side_solver_eff.nu_at
-          (compile_prog inc_pi [''p''] (IMP2_Proc.Call None ''p'' []))
+          (compile_prog inc_pi [''p''] (imp \<lbrakk> p() \<rbrakk>))
           sign_etf bot sign_init_s0 ()
-          (cfg_exit (compile_prog inc_pi [''p''] (IMP2_Proc.Call None ''p'' []))))
+          (cfg_exit (compile_prog inc_pi [''p''] (imp \<lbrakk> p() \<rbrakk>))))
        (td_cfg_side_solver_eff.stabl_at
-          (compile_prog inc_pi [''p''] (IMP2_Proc.Call None ''p'' []))
+          (compile_prog inc_pi [''p''] (imp \<lbrakk> p() \<rbrakk>))
           sign_etf bot sign_init_s0 ()
-          (cfg_exit (compile_prog inc_pi [''p''] (IMP2_Proc.Call None ''p'' []))))"
+          (cfg_exit (compile_prog inc_pi [''p''] (imp \<lbrakk> p() \<rbrakk>))))"
 proof -
   note result = mixed_flow_analysis_optimal
     [OF refl refl sign_sound_etf sign_etf_threefold_mono sign_etf_cone_compatible
         dom S_sound]
-  show "ltr_collect (compile_prog inc_pi [''p''] (IMP2_Proc.Call None ''p'' [])) S
-          (cfg_exit (compile_prog inc_pi [''p''] (IMP2_Proc.Call None ''p'' [])))
-        \<le> \<lbrakk>side_analyse_eff inc_pi [''p''] (IMP2_Proc.Call None ''p'' []) sign_etf
+  show "ltr_collect (compile_prog inc_pi [''p''] (imp \<lbrakk> p() \<rbrakk>)) S
+          (cfg_exit (compile_prog inc_pi [''p''] (imp \<lbrakk> p() \<rbrakk>)))
+        \<le> \<lbrakk>side_analyse_eff inc_pi [''p''] (imp \<lbrakk> p() \<rbrakk>) sign_etf
              bot sign_init_s0 ()
-             (cfg_exit (compile_prog inc_pi [''p''] (IMP2_Proc.Call None ''p'' [])))\<rbrakk>"
+             (cfg_exit (compile_prog inc_pi [''p''] (imp \<lbrakk> p() \<rbrakk>)))\<rbrakk>"
     using result(1) .
   show "least_part_post_solution
-         (side_cfg_T_eff (compile_prog inc_pi [''p''] (IMP2_Proc.Call None ''p'' []))
+         (side_cfg_T_eff (compile_prog inc_pi [''p''] (imp \<lbrakk> p() \<rbrakk>))
             sign_etf bot sign_init_s0 ())
-         (cfg_exit (compile_prog inc_pi [''p''] (IMP2_Proc.Call None ''p'' [])))
+         (cfg_exit (compile_prog inc_pi [''p''] (imp \<lbrakk> p() \<rbrakk>)))
          (td_cfg_side_solver_eff.nu_at
-            (compile_prog inc_pi [''p''] (IMP2_Proc.Call None ''p'' []))
+            (compile_prog inc_pi [''p''] (imp \<lbrakk> p() \<rbrakk>))
             sign_etf bot sign_init_s0 ()
-            (cfg_exit (compile_prog inc_pi [''p''] (IMP2_Proc.Call None ''p'' []))))
+            (cfg_exit (compile_prog inc_pi [''p''] (imp \<lbrakk> p() \<rbrakk>))))
          (td_cfg_side_solver_eff.stabl_at
-            (compile_prog inc_pi [''p''] (IMP2_Proc.Call None ''p'' []))
+            (compile_prog inc_pi [''p''] (imp \<lbrakk> p() \<rbrakk>))
             sign_etf bot sign_init_s0 ()
-            (cfg_exit (compile_prog inc_pi [''p''] (IMP2_Proc.Call None ''p'' []))))"
+            (cfg_exit (compile_prog inc_pi [''p''] (imp \<lbrakk> p() \<rbrakk>))))"
     using result(2) .
 qed
 text \<open>
@@ -95,15 +95,15 @@ corollary sign_mixed_flow_sound_from_pp:
   fixes \<sigma> :: "pp + unit \<Rightarrow> sign abs_state" and S :: "store set"
   assumes pp:
     "part_post_solution
-       (side_cfg_T_eff (compile_prog inc_pi [''p''] (IMP2_Proc.Call None ''p'' []))
-          sign_etf bot sign_init_s0 ()) (cfg_exit (compile_prog inc_pi [''p''] (IMP2_Proc.Call None ''p'' []))) \<sigma> vars"
+       (side_cfg_T_eff (compile_prog inc_pi [''p''] (imp \<lbrakk> p() \<rbrakk>))
+          sign_etf bot sign_init_s0 ()) (cfg_exit (compile_prog inc_pi [''p''] (imp \<lbrakk> p() \<rbrakk>))) \<sigma> vars"
   assumes entry:
-    "S \<le> \<lbrakk>side_env \<sigma> (cfg_entry (compile_prog inc_pi [''p''] (IMP2_Proc.Call None ''p'' [])))\<rbrakk>"
+    "S \<le> \<lbrakk>side_env \<sigma> (cfg_entry (compile_prog inc_pi [''p''] (imp \<lbrakk> p() \<rbrakk>)))\<rbrakk>"
   assumes inr: "inr_slot_locals_bot \<sigma>"
   shows
-    "ltr_collect (compile_prog inc_pi [''p''] (IMP2_Proc.Call None ''p'' [])) S
-       (cfg_exit (compile_prog inc_pi [''p''] (IMP2_Proc.Call None ''p'' [])))
-     \<le> \<lbrakk>side_env \<sigma> (cfg_exit (compile_prog inc_pi [''p''] (IMP2_Proc.Call None ''p'' [])))\<rbrakk>"
+    "ltr_collect (compile_prog inc_pi [''p''] (imp \<lbrakk> p() \<rbrakk>)) S
+       (cfg_exit (compile_prog inc_pi [''p''] (imp \<lbrakk> p() \<rbrakk>)))
+     \<le> \<lbrakk>side_env \<sigma> (cfg_exit (compile_prog inc_pi [''p''] (imp \<lbrakk> p() \<rbrakk>)))\<rbrakk>"
   by (rule mixed_flow_analysis_sound
         [OF sign_sound_etf pp entry sign_etf_cone_compatible
             compile_prog_finite[THEN conjunct1]
@@ -111,3 +111,4 @@ corollary sign_mixed_flow_sound_from_pp:
             inr])
 
 end
+
