src/Examples/Interprocedural/Example_Side_Proc_Global.thy
@@ -35,14 +35,14 @@ theorem proc_global_side_sign_analysis:
   fixes s t :: store
   assumes s_sound: "s \<in> \<lbrakk>side_proc_global_s0\<rbrakk>"
   assumes collect_exit:
-    "t \<in> ltr_collect (compile_prog inc_pi [''p''] (IMP2_Proc.Call None ''p'' [])) {s}
-       (cfg_exit (compile_prog inc_pi [''p''] (IMP2_Proc.Call None ''p'' [])))"
+    "t \<in> ltr_collect (compile_prog inc_pi [''p''] ''main'' (imp \<lbrakk> p() \<rbrakk>)) {s}
+       (cfg_exit (compile_prog inc_pi [''p''] ''main'' (imp \<lbrakk> p() \<rbrakk>)))"
   assumes side_solve_dom:
-    "side_cfg_solve_dom_eff (compile_prog inc_pi [''p''] (IMP2_Proc.Call None ''p'' [])) sign_etf bot
+    "side_cfg_solve_dom_eff (compile_prog inc_pi [''p''] ''main'' (imp \<lbrakk> p() \<rbrakk>)) sign_etf bot
        side_proc_global_s0 ()
-       (cfg_exit (compile_prog inc_pi [''p''] (IMP2_Proc.Call None ''p'' [])))"
-  shows "t \<in> \<lbrakk>side_analyse_eff inc_pi [''p''] (IMP2_Proc.Call None ''p'' []) sign_etf bot side_proc_global_s0 ()
-         (cfg_exit (compile_prog inc_pi [''p''] (IMP2_Proc.Call None ''p'' [])))\<rbrakk>"
+       (cfg_exit (compile_prog inc_pi [''p''] ''main'' (imp \<lbrakk> p() \<rbrakk>)))"
+  shows "t \<in> \<lbrakk>side_analyse_eff inc_pi [''p''] (imp \<lbrakk> p() \<rbrakk>) sign_etf bot side_proc_global_s0 ()
+         (cfg_exit (compile_prog inc_pi [''p''] ''main'' (imp \<lbrakk> p() \<rbrakk>)))\<rbrakk>"
   by (rule side_sign_analysis_sound[OF s_sound collect_exit side_solve_dom])
 subsection \<open>Executable sign analysis\<close>
 
@@ -51,9 +51,9 @@ definition inc_procs :: "pname list" where
 
 
 definition inc_main :: com where
-  "inc_main = IMP2_Proc.Call None ''p'' []"
+  "inc_main = imp \<lbrakk> p() \<rbrakk>"
 definition inc_prog :: imp_prog where
-  "inc_prog = imp_prog.make inc_procs inc_pi inc_main"
+  "inc_prog = imp_prog.make [(''p'', the (inc_pi ''p''))] inc_main"
 
 
 value "sign_exec_prog inc_prog ''Gx''"
@@ -83,3 +83,4 @@ ML_val \<open>
 \<close>
 
 end
+
